impl/fs/bilby/proof/adt/BufferT.thy
@@ -75,7 +75,7 @@ lemmas buf_simps = buf_take_def buf_drop_def buf_slice_def
 
 lemma drop_take_drop:
   "n \<le> m \<Longrightarrow> drop n (take m xs) @ drop m xs = drop n xs"
- by (metis Nat.le_iff_add add.commute take_drop take_drop_append)
+ by (metis add.commute atd_lem drop_drop drop_take le_add_diff_inverse)
 
 lemma buf_memset_bound_assm_eq:
   "unat (bound\<^sub>f buf) \<le>  length (\<alpha>wa (data\<^sub>f buf)) \<Longrightarrow>
