impl/fs/bilby/proof/lib/L4vBucket.thy
@@ -10,7 +10,8 @@
 
 theory L4vBucket
 imports
-  "../../../../../l4v/lib/WordLemmaBucket"
+  "Word_Lib.Word_Lemmas"
+  "../../../../../cogent/isa/Util"
 begin
 
 no_notation fun_app (infixr "$" 10)
@@ -31,7 +32,7 @@ lemma complement_mask:
   "complement (2 ^ n - 1) = ~~ mask n"
   unfolding complement_def mask_def
   by simp
-  
+
 lemma alignUp_idem:
   fixes a :: "'a::len word"
   assumes al: "is_aligned a n"
@@ -50,8 +51,8 @@ lemma alignUp_idem:
    apply simp
   apply (subst unat_sub)
    apply (subst unat_arith_simps)
-   apply (simp add: word_bits_def)
-  apply (simp add: word_bits_def del: unat_1)
+   apply (simp add: word_size)
+  apply (simp add: word_size del: unat_1)
   apply simp
   done
 
@@ -60,57 +61,8 @@ lemma alignUp_not_aligned_eq:
   assumes al: "\<not> is_aligned a n"
   and     sz: "n < len_of TYPE('a)"
   shows   "alignUp a n = (a div 2 ^ n + 1) * 2 ^ n"
-proof -
-  have anz: "a mod 2 ^ n \<noteq> 0" 
-    by (rule not_aligned_mod_nz) fact+
-  
-  hence um: "unat (a mod 2 ^ n - 1) div 2 ^ n = 0" using sz
-    apply -
-    apply (rule div_less)
-    apply (simp add: unat_minus_one del: word_neq_0_conv)
-    apply (rule order_less_trans)
-     apply (rule diff_Suc_less)
-     apply (erule contrapos_np)
-     apply (simp add: unat_eq_zero)
-    apply (subst unat_power_lower [symmetric, OF sz[unfolded word_bits_def]])  
-    apply (subst word_less_nat_alt [symmetric])
-    apply (rule word_mod_less_divisor)
-    apply (simp add: p2_gt_0)
-    done
-    
-  have "a + 2 ^ n - 1 = (a div 2 ^ n) * 2 ^ n + (a mod 2 ^ n) + 2 ^ n - 1"
-    by (simp add: word_mod_div_equality)
-  also have "\<dots> = (a mod 2 ^ n - 1) + (a div 2 ^ n + 1) * 2 ^ n"
-    by (simp add: field_simps)
-  finally show "alignUp a n = (a div 2 ^ n + 1) * 2 ^ n" using sz    
-    unfolding alignUp_def
-    apply (subst complement_mask)
-    apply (erule ssubst)
-    apply (subst neg_mask_is_div)
-    apply (simp add: word_arith_nat_div)
-    apply (subst unat_word_ariths(1) unat_word_ariths(2))+
-    apply (subst uno_simps)
-    apply (subst unat_1)
-    apply (subst mod_add_right_eq [symmetric])
-    apply (simp add: unat_power_lower)
-    apply (subst power_mod_div)
-    apply (subst div_mult_self1)
-    apply simp
-    apply (subst um)
-    apply simp
-    apply (subst mod_mod_power)
-    apply simp
-    apply (subst word_unat_power, subst Abs_fnat_hom_mult)
-    apply (subst mult_mod_left)
-    apply (subst power_add [symmetric])
-    apply simp
-    apply (subst Abs_fnat_hom_1)
-    apply (subst Abs_fnat_hom_add)
-    apply (subst word_unat_power, subst Abs_fnat_hom_mult)
-    apply (subst word_unat.Rep_inverse[symmetric], subst Abs_fnat_hom_mult)
-    apply simp
-    done
-qed
+  using assms
+  by (metis alignUp_not_aligned_eq)
 
 lemma alignUp_ge:
   fixes a :: "'a :: len word"
@@ -278,7 +230,7 @@ next
       apply (clarsimp simp: field_simps)
       apply (rule ccontr)
       apply (drule (1) order_le_neq_trans)
-      apply (simp add: unat_power_lower)
+      apply (force simp add: unat_power_lower)
       done
     
     hence "2 ^ (len_of TYPE('a) - n) - 1 < k" using r
